WIP on Record verification

src/tls/Record.fst
@@ -2,74 +2,104 @@ module Record
 
 (* (optional) encryption and processing of the outer (untrusted) record format *)
 
-open FStar.Seq
-open Platform.Bytes
+//open FStar.Seq
+open FStar.Bytes
 open FStar.Error
 
+open Mem
 open TLSError
 open TLSInfo
 open TLSConstants
+open Range
 open Content
+
+module HS = FStar.HyperStack
+module ST = FStar.HyperStack.ST
 
 // Consider merging some of this module with Content?
 
 (* A flag for runtime debugging of record data.
    The F* normalizer will erase debug prints at extraction
    when this flag is set to false. *)
-val discard: bool -> ST unit
+private val discard: bool -> ST unit
   (requires (fun _ -> True))
   (ensures (fun h0 _ h1 -> h0 == h1))
-let discard _ = ()
-let print s = discard (IO.debug_print_string ("REC| "^s^"\n"))
-unfold val trace: s:string -> ST unit
+private let discard _ = ()
+private let print s = discard (IO.debug_print_string ("REC| "^s^"\n"))
+private unfold val trace: s:string -> ST unit
   (requires (fun _ -> True))
   (ensures (fun h0 _ h1 -> h0 == h1))
-unfold let trace = if Flags.debug_Record then print else (fun _ -> ())
+private unfold let trace = if Flags.debug_Record then print else (fun _ -> ())
+
+
+assume val p_of_f: f:bytes -> p:Platform.Bytes.bytes { Platform.Bytes.length p = FStar.Bytes.length f } 
+assume val f_of_p: p:Platform.Bytes.bytes -> f:bytes { Platform.Bytes.length p = FStar.Bytes.length f } 
+let ctBytes x = f_of_p (ctBytes x)
+let parseCT (x: lbytes 1) = parseCT (p_of_f x)
+let versionBytes x = f_of_p (versionBytes x) 
+let parseVersion (x: lbytes 2) = parseVersion (p_of_f x)
 
 // ------------------------outer packet format -------------------------------
 
 // the "outer" header has the same format for all versions of TLS
 // but TLS 1.3 fakes its content type and protocol version.
 
-let x = Transport.recv
 
-type header = b:lbytes 5 // for all TLS versions
+// inline_for_extraction let x = Transport.recv
 
-let fake = ctBytes Application_data @| versionBytes TLS_1p0 
+private type header = b:lbytes 5 // for all TLS versions
+
+private let fake = ctBytes Application_data @| versionBytes TLS_1p2
 
 // this is the outer packet; the *caller* should switch from 1.3 to 1.0 whenever data is encrypted.
+private inline_for_extraction 
+let makeHeader ct plain ver (length:nat {repr_bytes length <= 2}): header =
+  let ct_ver = 
+    if TLS_1p3? ver then if plain then 
+      (ctBytes ct @| versionBytes TLS_1p2) 
+    else 
+      fake 
+    else 
+      (ctBytes ct @| versionBytes ver) in
+  ct_ver @| bytes_of_int 2 length 
+
+// used only for testing
 let makePacket ct plain ver (data: b:bytes { repr_bytes (length b) <= 2}) =
-  let header =
-    (if ver = TLS_1p3 then
-      (if plain then ctBytes ct @| versionBytes TLS_1p0
-       else fake)
-     else (ctBytes ct @| versionBytes ver))
-//      ctBytes ct 
-//   @| versionBytes ver
-   @| bytes_of_int 2 (length data) in
+  makeHeader ct plain ver (length data) @| data
+
+let sendPacket tcp ct plain ver (data: b:bytes { repr_bytes (length b) <= 2}) =
+  // still some margin for progress to avoid intermediate copies
+  let header = makeHeader ct plain ver (length data) in 
   trace ("record headers: "^print_bytes header);
-  header @| data 
+  let res = Transport.send tcp (BufferBytes.from_bytes header) 5ul in
+  if res = 5l then 
+    let res = Transport.send tcp (BufferBytes.from_bytes data) (len data) in
+    if Int32.v res = length data
+    then Correct()
+    else Error(Printf.sprintf "Transport.send returned %l" res)
+  else   Error(Printf.sprintf "Transport.send returned %l" res)
 
-
-val parseHeader: h5:header -> Tot (result (contentType 
-                                         * protocolVersion 
-                                         * l:nat { l <= max_TLSCiphertext_fragment_length}))
+type parsed_header = result (contentType
+                           * protocolVersion
+                           * l:nat { l <= max_TLSCiphertext_fragment_length})
+private val parseHeader: h5:header -> Tot parsed_header
 let parseHeader (h5:header) =
-    let (ct1,b4)   = Platform.Bytes.split h5 1 in
-    let (pv2,len2) = Platform.Bytes.split b4 2 in
+    let (ct1,b4)   = FStar.Bytes.split h5 1ul in
+    let (pv2,len2) = FStar.Bytes.split b4 2ul in
     match parseCT ct1 with
     | Error z -> Error z
     | Correct ct ->
-      match TLSConstants.parseVersion pv2 with
+      match parseVersion pv2 with
       | Error z -> Error z
       | Correct (UnknownVersion _ _) ->
         Error(AD_decode_error, perror __SOURCE_FILE__ __LINE__ "Parsed unknown protocol version")
       | Correct pv ->
           let len = int_of_bytes len2 in
-          if len <= 0 || len > max_TLSCiphertext_fragment_length 
+          if len <= 0 || len > max_TLSCiphertext_fragment_length
           then Error(AD_illegal_parameter, perror __SOURCE_FILE__ __LINE__ "Wrong fragment length")
           else correct(ct,pv,len)
 
+(*
 // hopefully we only care about the writer, not the cn state
 // the postcondition is of the form
 //   authId i ==> f is added to the writer log
@@ -84,7 +114,7 @@ let recordPacketOut (i:StatefulLHAE.id) (wr:StatefulLHAE.writer i) (pv: protocol
         StatefulLHAE.encrypt #i wr ad rg f
     in
     makePacket ct (PlaintextID? i) pv payload
-
+*)
 
 (*** networking (floating) ***)
 
@@ -93,69 +123,143 @@ let recordPacketOut (i:StatefulLHAE.id) (wr:StatefulLHAE.writer i) (pv: protocol
 // our client never checks the consistency of the server's record pv.
 // (see earlier versions for the checks we used to perform)
 
-// connectlon-local input state
-// to be improved once we extract to C  
-type partial = 
-  | Header 
+// connection-local input state
+type partial =
+  | Header
   | Body: ct: contentType -> pv: protocolVersion -> partial
-type input_state = 
-  | State:
-    waiting: nat {waiting>0} -> 
-    received: bytes -> 
-    st: partial {
-      match st with 
-      | Header -> length received + waiting = 5 
-      | Body _ _ -> length received + waiting <= max_TLSCiphertext_fragment_length } ->
-    input_state
-let wait_header = 
-  let data = empty_bytes in
-  assert(length empty_bytes = 0);
-  State 5 empty_bytes Header
 
-type read_result = 
+open FStar.UInt32
+
+private let maxlen = UInt32.uint_to_t (5 + max_TLSCiphertext_fragment_length)
+
+private type input_buffer =
+  b: Buffer.buffer UInt8.t {Buffer.length b = v maxlen}
+
+//TODO index by region
+noeq type input_state = | InputState:
+  pos: ref (len:UInt32.t {len <=^ maxlen}) ->
+  b: input_buffer {Buffer.frameOf b = Mem.frameOf pos}
+  -> input_state
+
+private let parseHeaderBuffer (b: Buffer.buffer UInt8.t {Buffer.length b = 5}) : ST parsed_header
+  (requires (fun h0 -> Buffer.live h0 b))
+  (ensures (fun h0 hdr h1 -> modifies_none h0 h1 /\ hdr = parseHeader (Bytes.hide (Buffer.as_seq h0 b))))
+=
+  // some margin for progress
+  parseHeader (BufferBytes.to_bytes 5 b)
+
+private let input_inv h0 (s: input_state) = 
+  Mem.contains h0 s.pos /\
+  Buffer.live h0 s.b /\
+  ( let pv = UInt32.v (sel h0 s.pos) in 
+    5 <= pv ==> (
+    match parseHeader (Bytes.hide (Buffer.as_seq h0 (Buffer.sub s.b 0ul 5ul))) with
+    | Correct (_,_,length) -> pv <= 5 + length
+    | _ -> False))
+
+private val waiting_len:  s: input_state -> ST UInt32.t
+  (requires fun h0 -> input_inv h0 s)
+  (ensures fun h0 len h1 -> 
+    modifies_none h0 h1 /\ 
+    ( let pv = UInt32.v (sel h0 s.pos) in 
+      let l = UInt32.v len in 
+      ( pv + l = 5 \/ 
+        ( match parseHeader (Bytes.hide (Buffer.as_seq h0 (Buffer.sub s.b 0ul 5ul))) with
+        | Correct (_,_,length) -> pv + l == 5 + length 
+        | _ -> False))))
+
+let waiting_len s =
+  if !s.pos <^ 5ul
+  then 5ul -^ !s.pos
+  else
+    match parseHeaderBuffer (Buffer.sub s.b 0ul 5ul) with
+    | Correct (_,_,length) -> 5ul +^ uint_to_t length -^ !s.pos
+      //let pv = UInt32.v !s.pos in 
+      //assert(length <= max_TLSCiphertext_fragment_length);
+      //assert(pv <= 5 + length);
+      //assert(FStar.UInt.size(length + 5) 32);
+      //assert(FStar.UInt.size(length + 5 - pv) 32);
+     // other case is statically excluded
+
+val alloc_input_state: r:_ -> ST input_state 
+  (requires (fun h0 -> is_eternal_region r))
+  (ensures (fun h0 s h1 ->
+    //TODO modifies? h0 h1 /\ 
+    Mem.frameOf s.pos = r /\ 
+    input_inv h1 s))
+let alloc_input_state r = 
+  let pos = ralloc r 0ul in 
+  let b = Buffer.rcreate r 0uy maxlen in
+  InputState pos b
+
+type read_result =
   | ReadError of TLSError.error
   | ReadWouldBlock
   | Received:
-      ct:contentType -> 
+      ct:contentType ->
       pv:protocolVersion ->
       b:bytes {length b <= max_TLSCiphertext_fragment_length} -> read_result
 
-val read: Transport.t -> s: HyperStack.ref input_state -> ST read_result
-  (requires fun h0 -> HyperStack.contains h0 s)
-  (ensures fun h0 _ h1 -> 
-    let id = HyperStack.frameOf s in 
-    HyperStack.modifies_one id h0 h1 /\ 
-    HyperStack.modifies_ref id (Set.singleton (HyperStack.as_addr s)) h0 h1 )
+val read: Transport.t -> s: input_state -> ST read_result
+  (requires fun h0 -> input_inv h0 s)
+  (ensures fun h0 _ h1 ->
+    let r = Mem.frameOf s.pos in
+    // Mem.modifies_one r h0 h1 /\
+    input_inv h1 s
+  )
+// Refine by adding this?
+//    Buffer.modifies_bufs_and_refs
+//      (Buffer.only s.b)
+//      (Set.singleton (Heap.addr_of (HS.as_ref s.pos)))
+//      h0 h1)
 
-let rec read tcp state =
-  let State len prior partial = !state in 
-  match Transport.recv tcp len with 
-  | Platform.Tcp.RecvWouldBlock -> trace "WouldBlock"; ReadWouldBlock
-  | Platform.Tcp.RecvError e -> ReadError (AD_internal_error, e) 
-  | Platform.Tcp.Received fresh -> (
-    let data = prior @| fresh in 
-    if length fresh = 0 then 
-      ReadError(AD_internal_error,"TCP close") // otherwise we loop...
-    else if length fresh < len then (
-      // partial read
-      state := State (len - length fresh) data partial; 
-      read tcp state // should probably ReadWouldBlock instead when non-blocking
-      )
-    else (
-      // we have received what we asked for
-      match partial with 
-      | Header -> (
-          match parseHeader data with  
-          | Error e -> ReadError e 
-          | Correct (ct,pv,len) -> 
-              if len = 0 then (
-                // corner case, possibly excluded by the RFC?
-                state := State 5 empty_bytes Header; 
-                Received ct pv empty_bytes )
-              else (
-                state := State  len empty_bytes (Body ct pv);
-                read tcp state ))
-      | Body ct pv -> (
-              state := State 5 empty_bytes Header; 
-              Received ct pv data )))
+#set-options "--detail_errors"
+let rec read tcp s =
+  let h0 = ST.get() in 
+  assert(input_inv h0 s);
+  let waiting = waiting_len s in
+  let p0 = !s.pos in
+  let dest = Buffer.sub s.b p0 waiting in
+  let res = Transport.recv tcp dest waiting in
+  let h1 = ST.get() in 
+  let p1 = !s.pos in 
+  assert(p0 = p1);
+  assume(input_inv h1 s);// TODO sub-buffer framing, with 2 cases
+  if res = -1l
+  then ReadError (AD_internal_error, "Transport.recv")
+  else if res = 0l
+  then (trace "WouldBlock"; ReadWouldBlock)
+  else (
+    let received = Int.Cast.int32_to_uint32 res in
+    assert(received <=^ waiting);
+    assert(UInt32.v p0 + UInt32.v waiting <= UInt32.v maxlen);
+    s.pos := p0 +^ received;
+    if received <^ waiting
+      then
+        // partial read
+        // should probably ReadWouldBlock instead when non-blocking
+        read tcp s
+      else
+        if !s.pos = 5ul // we have buffered the record header
+        then (
+          match parseHeaderBuffer s.b with
+          | Error e -> ReadError e
+          | Correct(ct,pv,length) ->
+            if length = 0 then
+              // corner case, possibly excluded by the RFC
+              ( s.pos := 0ul; Received ct pv empty_bytes )
+            else read tcp s )
+        else
+          // we have buffered the whole record
+          match parseHeaderBuffer s.b with
+          | Correct(ct,pv,length) -> (
+            let len = UInt32.uint_to_t length in
+            let b = Buffer.sub s.b 5ul len in
+            let payload = BufferBytes.to_bytes length b in
+            s.pos := 0ul;
+            Received ct pv payload ))
+
+//18-01-24 recheck async I
+//    if length fresh = 0 then
+//      ReadError(AD_internal_error,"TCP close") // otherwise we loop...
 
