src/tls/Transport.fst
@@ -2,64 +2,84 @@ module Transport
 
 // adding an indirection to TCP for applications that prefer to take control of their IOs.
 
-open Platform.Tcp 
-open Platform.Bytes
+open FStar.Bytes
 open FStar.Error
 open TLSError
-
 open Mem
 
 
-// make this type abstract? 
-noeq type t = { 
-  snd: bytes -> ST (optResult string unit) (fun _ -> True) (fun h0 _ h1 -> h0 == h1);
-  rcv: max:nat -> ST (recv_result max) (fun _ -> True) (fun h0 _ h1 -> h0 == h1) }
+/// 18-01-23 We now have function pointers matching the types used in
+/// mitls.h. After hoisting for Kremlin extraction, we treat the
+/// explicit context as a dyn to avoid climbing in universes.
 
-let callbacks send recv = { snd = send; rcv = recv } 
+type pvoid = FStar.Dyn.dyn
+type size_t = UInt32.t 
+type pfn_send = 
+  pvoid -> 
+  output_buffer: FStar.Buffer.buffer UInt8.t -> 
+  max_len: size_t -> ST Int32.t
+  (requires fun h0 -> 
+    Buffer.live h0 output_buffer /\ 
+    UInt32.v max_len = Buffer.length output_buffer)
+  (ensures fun h0 r h1 -> 
+    let v = Int32.v r in
+    modifies_none h0 h1 /\
+    (v = -1 \/ (0 <= v /\ v <= UInt32.v max_len)))
 
-// platform implementation
+type pfn_recv = 
+  pvoid -> 
+  input_buffer: FStar.Buffer.buffer UInt8.t -> 
+  max_len: size_t -> ST Int32.t
+  (requires fun h0 ->
+    Buffer.live h0 input_buffer /\
+    UInt32.v max_len = Buffer.length input_buffer)
+  (ensures fun h0 r h1 -> 
+    let v = Int32.v r in 
+    Buffer.modifies_1 input_buffer h0 h1 /\ 
+    (v = -1 \/ (0 <= v /\ v <= UInt32.v max_len)))
+    
+noeq type t = {
+  ptr : pvoid;
+  snd: pfn_send;
+  rcv: pfn_recv }
 
-let wrap tcp: t = callbacks (send tcp) (recv_async tcp)
-type tcpListener = tcpListener
+let callbacks v send recv: t = { ptr = v; snd = send; rcv = recv }
 
-let listen domain port : ML tcpListener = listen domain port
-let accept listener = wrap (accept listener)
-let connect domain port = wrap (connect domain port)
-let close = close
+// following the indirection
+let send t buffer len = t.snd t.ptr buffer len 
+let recv t buffer len = t.rcv t.ptr buffer len 
 
-// following the indirection 
-
-let send tcp data = tcp.snd data
-let recv tcp len = tcp.rcv len
-
-val test: t -> bytes -> ML unit
-let test (tcp:t) (data:bytes) = 
-  let h0 = get() in 
-  let _ = tcp.snd data in
-  let h1 = get() in 
-  assert (h0==h1)
-  
-
+// val test: t -> b: Buffer.buffer UInt8.t {Buffer.length b = 5} -> ST unit
+//   (requires fun h0 -> Buffer.live h0 b)
+//   (ensures fun h0 r h1 -> h0 == h1)
+// let test t b =
+//   let _ = send t b 5ul in
+//   ()
 
 // for now we get a runtime error in case of partial write on an asynchronous socket
 
+(* 18-01-23 not used in quic2c? 
 
 // forces read to complete, even if the socket is non-blocking.
 // this may cause spinning.
 
-private val really_read_rec: b:bytes -> t -> l:nat -> ST (recv_result (l+length b))
+private val really_read_rec: b:bytes -> t 'a -> l:nat -> ST (recv_result (l+length b))
   (fun _ -> True) (fun h0 _ h1 -> h0 == h1)
-let rec really_read_rec prev tcp len = 
-    if len = 0 
+let rec really_read_rec prev tcp len =
+    if len = 0
     then Received prev
-    else 
+    else
       match recv tcp len with
       | RecvWouldBlock -> really_read_rec prev tcp len
-      | Received b -> 
+      | Received b ->
             let lb = length b in
-      	    if lb = len then Received(prev @| b)
-      	    else if lb = 0 then RecvError "TCP close" //16-07-24 otherwise we loop...
+            if lb = len then Received(prev @| b)
+            else if lb = 0 then RecvError "TCP close" //16-07-24 otherwise we loop...
             else really_read_rec (prev @| b) tcp (len - lb)
       | RecvError e -> RecvError e
 
 let really_read = really_read_rec empty_bytes
+*)
+
+
+
